Separate Inst.toFormat

RV32I/Def.lean
@@ -1,216 +1,447 @@
-/-! # Chapter 34. RV32/64G Instruction Set Listings
+import Mathlib.Data.Fin.VecNotation
+import Mathlib.Logic.Equiv.Defs
+import Mathlib.Tactic.FinCases
 
+/-! # Chapter 2. Inst Base Integer Instruction Set, Version 2.1
+
+## Chapter 34. RV32/64G Instruction Set Listings
 The [ascii doc source](https://github.com/riscv/riscv-isa-manual/blob/main/src/rv-32-64g.adoc).
-
-## RV32I Base Instruction Set
 
 -/
 
-inductive Rtype
-  : (funct7 : BitVec 7)
-  → (rs2    : BitVec 5)
-  → (rs1    : BitVec 5)
-  → (funct3 : BitVec 3)
-  → (rd     : BitVec 5)
-  → (opcode : BitVec 7)
-  → Type
-  | SLLI shamt rs1 rd : Rtype 0b0000000 shamt rs1 0b001 rd 0b0010011
-  | SRLI shamt rs1 rd : Rtype 0b0000000 shamt rs1 0b101 rd 0b0010011
-  | SRAI shamt rs1 rd : Rtype 0b0100000 shamt rs1 0b101 rd 0b0010011
-  | ADD  rs2   rs1 rd : Rtype 0b0000000 rs2   rs1 0b000 rd 0b0110011
-  | SUB  rs2   rs1 rd : Rtype 0b0100000 rs2   rs1 0b000 rd 0b0110011
-  | SLL  rs2   rs1 rd : Rtype 0b0000000 rs2   rs1 0b001 rd 0b0110011
-  | SLT  rs2   rs1 rd : Rtype 0b0000000 rs2   rs1 0b010 rd 0b0110011
-  | SLTU rs2   rs1 rd : Rtype 0b0000000 rs2   rs1 0b011 rd 0b0110011
-  | XOR  rs2   rs1 rd : Rtype 0b0000000 rs2   rs1 0b100 rd 0b0110011
-  | SRL  rs2   rs1 rd : Rtype 0b0000000 rs2   rs1 0b101 rd 0b0110011
-  | SRA  rs2   rs1 rd : Rtype 0b0100000 rs2   rs1 0b101 rd 0b0110011
-  | OR   rs2   rs1 rd : Rtype 0b0000000 rs2   rs1 0b110 rd 0b0110011
-  | AND  rs2   rs1 rd : Rtype 0b0000000 rs2   rs1 0b111 rd 0b0110011
+/-! ## 2.1. Programmers' Model for Base Integer ISA
+-/
 
-inductive Itype
-  : («imm[11:0]» : BitVec 12)
-  → (rs1         : BitVec  5)
-  → (funct3      : BitVec  3)
-  → (rd          : BitVec  5)
-  → (opcode      : BitVec  7)
-  → Type
-  | JALR  «imm[11:0]» rs1 rd : Itype «imm[11:0]» rs1 0b000 rd 0b1100111
-  | LB    «imm[11:0]» rs1 rd : Itype «imm[11:0]» rs1 0b000 rd 0b0000011
-  | LH    «imm[11:0]» rs1 rd : Itype «imm[11:0]» rs1 0b001 rd 0b0000011
-  | LW    «imm[11:0]» rs1 rd : Itype «imm[11:0]» rs1 0b010 rd 0b0000011
-  | LBU   «imm[11:0]» rs1 rd : Itype «imm[11:0]» rs1 0b100 rd 0b0000011
-  | LHU   «imm[11:0]» rs1 rd : Itype «imm[11:0]» rs1 0b101 rd 0b0000011
-  | ADDI  «imm[11:0]» rs1 rd : Itype «imm[11:0]» rs1 0b000 rd 0b0010011
-  | SLTI  «imm[11:0]» rs1 rd : Itype «imm[11:0]» rs1 0b010 rd 0b0010011
-  | SLTIU «imm[11:0]» rs1 rd : Itype «imm[11:0]» rs1 0b011 rd 0b0010011
-  | XORI  «imm[11:0]» rs1 rd : Itype «imm[11:0]» rs1 0b100 rd 0b0010011
-  | ORI   «imm[11:0]» rs1 rd : Itype «imm[11:0]» rs1 0b110 rd 0b0010011
-  | ANDI  «imm[11:0]» rs1 rd : Itype «imm[11:0]» rs1 0b111 rd 0b0010011
-  | FENCE (fm pred succ : BitVec 4) rs1 rd : Itype (fm ++ pred ++ succ) rs1 0b000 rd 0b0001111
-  | FENCE.TSO : Itype (0b1000#4 ++ 0b0011#4 ++ 0b0011#4) 0b00000 0b000 0b00000 0b0001111
-  | PAUSE     : Itype (0b0000#4 ++ 0b0001#4 ++ 0b0000#4) 0b00000 0b000 0b00000 0b0001111
-  | ECALL     : Itype 0b000000000000 0b00000 0b000 0b00000 0b1110011
-  | EBREAK    : Itype 0b000000000001 0b00000 0b000 0b00000 0b1110011
+inductive Reg
+  /-- Zero. Immutable. -/
+  | zero
+  /-- Return address. -/
+  | ra
+  /-- Stack pointer. Preserved across calls. -/
+  | sp
+  /-- Global pointer. Unallocatable. -/
+  | gp
+  /-- Thread pointer. Unallocatable. -/
+  | tp
+  /-- Temporary registers. -/
+  | t (i : Fin 7)
+  /-- Callee-saved registers. Preserved across calls. -/
+  | s (i : Fin 12)
+  /-- Argument registers. -/
+  | a (i : Fin 8)
 
-inductive Stype
-  : («imm[11:5]» : BitVec 7)
-  → (rs2         : BitVec 5)
-  → (rs1         : BitVec 5)
-  → (funct3      : BitVec 3)
-  → («imm[4:0]»  : BitVec 5)
-  → (opcode      : BitVec 7)
-  → Type
-  | SB «imm[11:5]» rs2 rs1 «imm[4:0]» : Stype «imm[11:5]» rs2 rs1 0b000 «imm[4:0]» 0b0100011
-  | SH «imm[11:5]» rs2 rs1 «imm[4:0]» : Stype «imm[11:5]» rs2 rs1 0b001 «imm[4:0]» 0b0100011
-  | SW «imm[11:5]» rs2 rs1 «imm[4:0]» : Stype «imm[11:5]» rs2 rs1 0b010 «imm[4:0]» 0b0100011
+instance Reg.x : Equiv (Fin 32) Reg where
+  toFun
+  -- := ![
+  --   zero, ra, sp, gp, tp, t 0, t 1, t 2,
+  --   s 0, s 1, a 0, a 1, a 2, a 3, a 4, a 5,
+  --   a 6, a 7, s 2, s 3, s 4, s 5, s 6, s 7,
+  --   s 8, s 9, s 10, s 11, t 3, t 4, t 5, t 6
+  -- ]
+    | 0 => zero | 1 => ra | 2 => sp | 3 => gp | 4 => tp
+    | 5 => t 0 | 6 => t 1 | 7 => t 2
+    | 8 => s 0 | 9 => s 1
+    | 10 => a 0 | 11 => a 1 | 12 => a 2 | 13 => a 3 | 14 => a 4 | 15 => a 5
+      | 16 => a 6 | 17 => a 7
+    | 18 => s 2 | 19 => s 3 | 20 => s 4 | 21 => s 5 | 22 => s 6 | 23 => s 7
+      | 24 => s 8 | 25 => s 9 | 26 => s 10 | 27 => s 11
+    | 28 => t 3 | 29 => t 4 | 30 => t 5 | 31 => t 6
+    | ⟨n + 32, (h : n + 32 < 32)⟩ =>
+      absurd (Nat.le_add_left 32 n) (Nat.not_le_of_gt h)
+  invFun
+    | zero => 0 | ra => 1 | sp => 2 | gp => 3 | tp => 4
+    | t 0 => 5 | t 1 => 6 | t 2 => 7
+    | s 0 => 8 | s 1 => 9
+    | a ⟨n, _⟩ => n + 10
+    | s ⟨n + 2, _⟩ => n + 18
+    -- | t 3 => 28 | t 4 => 29 | t 5 => 30 | t 6 => 31
+    | t ⟨n + 3, _⟩ => n + 28
+  left_inv (i : Fin 32) := by fin_cases i <;> rfl
+  right_inv (x : Reg) := by
+    cases x <;> try rfl
+    case t i => fin_cases i <;> rfl
+    case s i => fin_cases i <;> rfl
+    case a i => fin_cases i <;> rfl
 
-inductive Btype
-  : («imm[12|10:5]» : BitVec 7)
-  → (rs2            : BitVec 5)
-  → (rs1            : BitVec 5)
-  → (funct3         : BitVec 3)
-  → («imm[4:1|11]»  : BitVec 5)
-  → (opcode         : BitVec 7)
-  → Type
-  | BEQ  «imm[12|10:5]» rs2 rs1 «imm[4:1|11]» : Btype «imm[12|10:5]» rs2 rs1 0b000 «imm[4:1|11]» 0b1100011
-  | BNE  «imm[12|10:5]» rs2 rs1 «imm[4:1|11]» : Btype «imm[12|10:5]» rs2 rs1 0b001 «imm[4:1|11]» 0b1100011
-  | BLT  «imm[12|10:5]» rs2 rs1 «imm[4:1|11]» : Btype «imm[12|10:5]» rs2 rs1 0b100 «imm[4:1|11]» 0b1100011
-  | BGE  «imm[12|10:5]» rs2 rs1 «imm[4:1|11]» : Btype «imm[12|10:5]» rs2 rs1 0b101 «imm[4:1|11]» 0b1100011
-  | BLTU «imm[12|10:5]» rs2 rs1 «imm[4:1|11]» : Btype «imm[12|10:5]» rs2 rs1 0b110 «imm[4:1|11]» 0b1100011
-  | BGEU «imm[12|10:5]» rs2 rs1 «imm[4:1|11]» : Btype «imm[12|10:5]» rs2 rs1 0b111 «imm[4:1|11]» 0b1100011
+instance : Coe Reg (BitVec 5) where
+  coe x := Reg.x.symm x
 
-inductive Utype
-  : («imm[31:12]» : BitVec 20)
-  → (rd           : BitVec  5)
-  → (opcode       : BitVec  7)
-  → Type
-  | LUI   «imm[31:12]» rd : Utype «imm[31:12]» rd 0b0110111
-  | AUIPC «imm[31:12]» rd : Utype «imm[31:12]» rd 0b0010111
+instance : Coe (BitVec 5) Reg where
+  coe i := Reg.x i.toFin
 
-inductive Jtype
-  : («imm[20|10:1|11|19:12]» : BitVec 20)
-  → (rd                      : BitVec  5)
-  → (opcode                  : BitVec  7)
-  → Type
-  | JAL «imm[20|10:1|11|19:12]» rd : Jtype «imm[20|10:1|11|19:12]» rd 0b1101111
+/-- Table 70. RISC-V base opcode map, `inst[1:0]=11`. -/
+inductive Opcode : Type
+  -- `inst[6:5]=00`
+  | LOAD | «LOAD-FP» | «custom-0» | «MISC-MEM» | «OP-IMM» | AUIPC | «OP-IMM-32» | «48b»
+  -- `inst[6:5]=01`
+  | STORE | «STORE-FP» | «custom-1» | AMO | OP | LUI | «OP-32» | «64b»
+  -- `inst[6:5]=10`
+  | MADD | MSUB | NMSUB | NMADD | «OP-FP» | «OP-V» | «custom-2/rv128»
+    /-- Rewritten as `48b` in the spec. -/ | «48b'»
+  -- `inst[6:5]=11`
+  | BRANCH | JALR | reserved | JAL | SYSTEM | «OP-VE» | «custom-3/rv128» | «≥80b»
+
+def Opcode.toBitVec : Opcode → BitVec 7
+  -- `inst[6:5]=00`
+  | LOAD             => 0b00_000_11
+  | «LOAD-FP»        => 0b00_001_11
+  | «custom-0»       => 0b00_010_11
+  | «MISC-MEM»       => 0b00_011_11
+  | «OP-IMM»         => 0b00_100_11
+  | AUIPC            => 0b00_101_11
+  | «OP-IMM-32»      => 0b00_110_11
+  | «48b»            => 0b00_111_11
+  -- `inst[6:5]=01`
+  | STORE            => 0b01_000_11
+  | «STORE-FP»       => 0b01_001_11
+  | «custom-1»       => 0b01_010_11
+  | AMO              => 0b01_011_11
+  | OP               => 0b01_100_11
+  | LUI              => 0b01_101_11
+  | «OP-32»          => 0b01_110_11
+  | «64b»            => 0b01_111_11
+  -- `inst[6:5]=10`
+  | MADD             => 0b10_000_11
+  | MSUB             => 0b10_001_11
+  | NMSUB            => 0b10_010_11
+  | NMADD            => 0b10_011_11
+  | «OP-FP»          => 0b10_100_11
+  | «OP-V»           => 0b10_101_11
+  | «custom-2/rv128» => 0b10_110_11
+  | «48b'»           => 0b10_111_11
+  -- `inst[6:5]=11`
+  | BRANCH           => 0b11_000_11
+  | JALR             => 0b11_001_11
+  | reserved         => 0b11_010_11
+  | JAL              => 0b11_011_11
+  | SYSTEM           => 0b11_100_11
+  | «OP-VE»          => 0b11_101_11
+  | «custom-3/rv128» => 0b11_110_11
+  | «≥80b»           => 0b11_111_11
+
+instance : Coe Opcode (BitVec 7) where
+  coe := Opcode.toBitVec
+
+theorem Opcode.toBitVec_lsbs_all_one (opcode : Opcode)
+  : opcode.toBitVec.extractLsb 1 0 = 0b11#2 := by cases opcode <;> trivial
+
+/-- 2.2. Base Instruction Formats -/
+class inductive Inst.Format
+  | Rtype
+    : (funct7       : BitVec  7)
+    → (rs2          : BitVec  5)
+    → (rs1          : BitVec  5)
+    → (funct3       : BitVec  3)
+    → (rd           : BitVec  5)
+    → Opcode → Format
+  | Itype
+    : («imm[11:0]»  : BitVec 12)
+    → (rs1          : BitVec  5)
+    → (funct3       : BitVec  3)
+    → (rd           : BitVec  5)
+    → Opcode → Format
+  | Stype
+    : («imm[11:5]»  : BitVec  7)
+    → (rs2          : BitVec  5)
+    → (rs1          : BitVec  5)
+    → (funct3       : BitVec  3)
+    → («imm[4:0]»   : BitVec  5)
+    → Opcode → Format
+  | Btype
+    : («imm[12]»    : BitVec  1)
+    → («imm[10:5]»  : BitVec  6)
+    → (rs2          : BitVec  5)
+    → (rs1          : BitVec  5)
+    → (funct3       : BitVec  3)
+    → («imm[4:1]»   : BitVec  4)
+    → («imm[11]»    : BitVec  1)
+    → Opcode → Format
+  | Utype
+    : («imm[31:12]» : BitVec 20)
+    → (rd           : BitVec  5)
+    → Opcode → Format
+  | Jtype
+    : («imm[20]»    : BitVec  1)
+    → («imm[10:1]»  : BitVec 10)
+    → («imm[11]»    : BitVec  1)
+    → («imm[19:12]» : BitVec  8)
+    → (rd           : BitVec  5)
+    → Opcode → Format
+
+namespace Inst.Format
+
+abbrev Rtype' funct7 rs2 rs1 funct3 rd :=
+  Rtype funct7 rs2 rs1 funct3 rd .OP
+
+/-- Shifts by a constant -/
+abbrev Itype' (funct7 : BitVec 7) (shamt : BitVec 5) rs1 funct3 rd :=
+  Itype (funct7 ++ shamt) rs1 funct3 rd .«OP-IMM»
+
+/-- `pred,succ = iorw` -/
+abbrev Mtype (fm pred succ : BitVec  4) rs1 funct3 rd :=
+  Itype (fm ++ pred ++ succ) rs1 funct3 rd .«MISC-MEM»
+
+abbrev Stype' (offset : BitVec 12) rs2 rs1 funct3 :=
+  Stype
+    (offset.extractLsb 11 5)
+    rs2 rs1 funct3
+    (offset.extractLsb  4 0)
+    .STORE
+
+abbrev Btype' (offset1 : BitVec 12) rs2 rs1 funct3 :=
+  Btype
+    (offset1.extractLsb 11 11)
+    (offset1.extractLsb  9  4)
+    rs2 rs1 funct3
+    (offset1.extractLsb  3  0)
+    (offset1.extractLsb 10 10)
+    .BRANCH
+
+abbrev Jtype' (offset1 : BitVec 20) rd :=
+  Jtype
+    (offset1.extractLsb 19 19)
+    (offset1.extractLsb  9  0)
+    (offset1.extractLsb 10 10)
+    (offset1.extractLsb 18 11)
+    rd .JAL
+
+def toUInt32 : Format → UInt32
+  | Rtype funct7 rs2 rs1 funct3 rd opcode =>
+    UInt32.mk <| funct7 ++ rs2 ++ rs1 ++ funct3 ++ rd ++ opcode.toBitVec
+  | Itype «imm[11:0]» rs1 funct3 rd opcode =>
+    UInt32.mk <| «imm[11:0]» ++ rs1 ++ funct3 ++ rd ++ opcode.toBitVec
+  | Stype «imm[11:5]» rs2 rs1 funct3 «imm[4:0]» opcode =>
+    UInt32.mk <| «imm[11:5]» ++ rs2 ++ rs1 ++ funct3 ++ «imm[4:0]» ++ opcode.toBitVec
+  | Btype «imm[12]» «imm[10:5]» rs2 rs1 funct3 «imm[4:1|11]» «imm[11]» opcode =>
+    UInt32.mk <| «imm[12]» ++ «imm[10:5]» ++ rs2 ++ rs1 ++ funct3 ++ «imm[4:1|11]» ++ «imm[11]» ++ opcode.toBitVec
+  | Utype «imm[31:12]» rd opcode =>
+    UInt32.mk <| «imm[31:12]» ++ rd ++ opcode.toBitVec
+  | Jtype «imm[20]» «imm[10:1]» «imm[11]» «imm[19:12]» rd opcode =>
+    UInt32.mk <| «imm[20]» ++ «imm[10:1]» ++ «imm[11]» ++ «imm[19:12]» ++ rd ++ opcode.toBitVec
+
+end Inst.Format
+
+/-! ## 2.4. Integer Computational Instructions
+
+No integer computational instructions cause arithmetic exceptions.
+-/
 
 inductive Inst
-  | ofRtype {funct7 rs2 rs1 funct3 rd opcode}
-    : Rtype funct7 rs2 rs1 funct3 rd opcode → Inst
-  | ofItype {«imm[11:0]» rs1 funct3 rd opcode}
-    : Itype «imm[11:0]» rs1 funct3 rd opcode → Inst
-  | ofStype {«imm[11:5]» rs2 rs1 funct3 «imm[4:0]» opcode}
-    : Stype «imm[11:5]» rs2 rs1 funct3 «imm[4:0]» opcode → Inst
-  | ofBtype {«imm[12|10:5]» rs2 rs1 funct3 «imm[4:1|11]» opcode}
-    : Btype «imm[12|10:5]» rs2 rs1 funct3 «imm[4:1|11]» opcode → Inst
-  | ofUtype {«imm[31:12]» rd opcode}
-    : Utype «imm[31:12]» rd opcode → Inst
-  | ofJtype {«imm[20|10:1|11|19:12]» rd opcode}
-    : Jtype «imm[20|10:1|11|19:12]» rd opcode → Inst
+  /- 2.4.1. Integer Register-Immediate Instructions -/
+  | ADDI  (rd rs1     : Reg) (imm   : BitVec 12)
+  | SLTI  (rd rs1     : Reg) (imm   : BitVec 12)
+  | SLTIU (rd rs1     : Reg) (imm   : BitVec 12)
+  | ANDI  (rd rs1     : Reg) (imm   : BitVec 12)
+  | ORI   (rd rs1     : Reg) (imm   : BitVec 12)
+  | XORI  (rd rs1     : Reg) (imm   : BitVec 12)
+  | SLLI  (rd rs1     : Reg) (shamt : BitVec  5)
+  | SRLI  (rd rs1     : Reg) (shamt : BitVec  5)
+  | SRAI  (rd rs1     : Reg) (shamt : BitVec  5)
+  | LUI   (rd         : Reg) (imm   : BitVec 20)
+  | AUIPC (rd         : Reg) (imm   : BitVec 20)
+  /- 2.4.2. Integer Register-Register Operations -/
+  | ADD   (rd rs1 rs2 : Reg)
+  | SLT   (rd rs1 rs2 : Reg)
+  | SLTU  (rd rs1 rs2 : Reg)
+  | AND   (rd rs1 rs2 : Reg)
+  | OR    (rd rs1 rs2 : Reg)
+  | XOR   (rd rs1 rs2 : Reg)
+  | SLL   (rd rs1 rs2 : Reg)
+  | SRL   (rd rs1 rs2 : Reg)
+  | SUB   (rd rs1 rs2 : Reg)
+  | SRA   (rd rs1 rs2 : Reg)
+  /- 2.5.1. Unconditional Jumps -/
+  | JAL   (rd         : Reg) (offset : BitVec 20)
+  | JALR  (rd rs1     : Reg) (offset : BitVec 12)
+  /- 2.5.2. Conditional Branches -/
+  | BEQ   (   rs1 rs2 : Reg) (offset : BitVec 12)
+  | BNE   (   rs1 rs2 : Reg) (offset : BitVec 12)
+  | BLT   (   rs1 rs2 : Reg) (offset : BitVec 12)
+  | BGE   (   rs1 rs2 : Reg) (offset : BitVec 12)
+  | BLTU  (   rs1 rs2 : Reg) (offset : BitVec 12)
+  | BGEU  (   rs1 rs2 : Reg) (offset : BitVec 12)
+  /- 2.6. Load and Store Instructions -/
+  | LW    (rd rs1     : Reg) (offset : BitVec 12)
+  | LH    (rd rs1     : Reg) (offset : BitVec 12)
+  | LHU   (rd rs1     : Reg) (offset : BitVec 12)
+  | LB    (rd rs1     : Reg) (offset : BitVec 12)
+  | LBU   (rd rs1     : Reg) (offset : BitVec 12)
+  | SW   (rs2 rs1     : Reg) (offset : BitVec 12)
+  | SH   (rs2 rs1     : Reg) (offset : BitVec 12)
+  | SB   (rs2 rs1     : Reg) (offset : BitVec 12)
+  /- 2.7. Memory Ordering Instructions -/
+  | FENCE (pred succ : BitVec 4)
+  | FENCE.TSO
+  /- 2.8. Environment Call and Breakpoints -/
+  | ECALL
+  | EBREAK
 
 namespace Inst
 
-open Rtype Itype Stype Btype Utype Jtype
+instance toFormat : Inst → Format
+  /- 2.4.1. Integer Register-Immediate Instructions -/
+  | ADDI  rd  rs1 imm    => .Itype  imm          rs1 0b000 rd .«OP-IMM»
+  | SLTI  rd  rs1 imm    => .Itype  imm          rs1 0b010 rd .«OP-IMM»
+  | SLTIU rd  rs1 imm    => .Itype  imm          rs1 0b011 rd .«OP-IMM»
+  | ANDI  rd  rs1 imm    => .Itype  imm          rs1 0b111 rd .«OP-IMM»
+  | ORI   rd  rs1 imm    => .Itype  imm          rs1 0b110 rd .«OP-IMM»
+  | XORI  rd  rs1 imm    => .Itype  imm          rs1 0b100 rd .«OP-IMM»
+  | SLLI  rd  rs1 shamt  => .Itype'      0 shamt rs1 0b001 rd
+  | SRLI  rd  rs1 shamt  => .Itype'      0 shamt rs1 0b101 rd
+  | SRAI  rd  rs1 shamt  => .Itype'     32 shamt rs1 0b101 rd
+  | LUI   rd      imm    => .Utype  imm                    rd .LUI
+  | AUIPC rd      imm    => .Utype  imm                    rd .AUIPC
+  /- 2.4.2. Integer Register-Register Operations -/
+  | ADD   rd  rs1 rs2    => .Rtype'      0 rs2   rs1 0b000 rd
+  | SLT   rd  rs1 rs2    => .Rtype'      0 rs2   rs1 0b010 rd
+  | SLTU  rd  rs1 rs2    => .Rtype'      0 rs2   rs1 0b011 rd
+  | AND   rd  rs1 rs2    => .Rtype'      0 rs2   rs1 0b111 rd
+  | OR    rd  rs1 rs2    => .Rtype'      0 rs2   rs1 0b110 rd
+  | XOR   rd  rs1 rs2    => .Rtype'      0 rs2   rs1 0b100 rd
+  | SLL   rd  rs1 rs2    => .Rtype'      0 rs2   rs1 0b001 rd
+  | SRL   rd  rs1 rs2    => .Rtype'      0 rs2   rs1 0b101 rd
+  | SUB   rd  rs1 rs2    => .Rtype'     32 rs2   rs1 0b000 rd
+  | SRA   rd  rs1 rs2    => .Rtype'     32 rs2   rs1 0b101 rd
+  /- 2.5.1. Unconditional Jumps -/
+  | JAL   rd      offset => .Jtype' offset                 rd
+  | JALR  rd  rs1 offset => .Itype  offset       rs1 0b000 rd .JALR
+  /- 2.5.2. Conditional Branches -/
+  | BEQ   rs1 rs2 offset => .Btype' offset rs2   rs1 0b000
+  | BNE   rs1 rs2 offset => .Btype' offset rs2   rs1 0b001
+  | BLT   rs1 rs2 offset => .Btype' offset rs2   rs1 0b100
+  | BGE   rs1 rs2 offset => .Btype' offset rs2   rs1 0b101
+  | BLTU  rs1 rs2 offset => .Btype' offset rs2   rs1 0b110
+  | BGEU  rs1 rs2 offset => .Btype' offset rs2   rs1 0b111
+  /- 2.6. Load and Store Instructions -/
+  | LW    rd  rs1 offset => .Itype  offset       rs1 0b010 rd .LOAD
+  | LH    rd  rs1 offset => .Itype  offset       rs1 0b001 rd .LOAD
+  | LHU   rd  rs1 offset => .Itype  offset       rs1 0b101 rd .LOAD
+  | LB    rd  rs1 offset => .Itype  offset       rs1 0b000 rd .LOAD
+  | LBU   rd  rs1 offset => .Itype  offset       rs1 0b100 rd .LOAD
+  | SW    rs2 rs1 offset => .Stype' offset rs2   rs1 0b010
+  | SH    rs2 rs1 offset => .Stype' offset rs2   rs1 0b001
+  | SB    rs2 rs1 offset => .Stype' offset rs2   rs1 0b000
+  /- 2.7. Memory Ordering Instructions -/
+  | FENCE pred succ      => .Mtype 0 pred   succ   0 0b000  0
+  | FENCE.TSO            => .Mtype 8 0b0011 0b0011 0 0b000  0
+  /- 2.8. Environment Call and Breakpoints -/
+  | ECALL                => .Itype              0  0 0b000  0 .SYSTEM
+  | EBREAK               => .Itype              1  0 0b000  0 .SYSTEM
 
-def toUInt32 : Inst → UInt32
-  | @ofRtype funct7 rs2 rs1 funct3 rd opcode _ =>
-    UInt32.mk <| funct7 ++ rs2 ++ rs1 ++ funct3 ++ rd ++ opcode
-  | @ofItype «imm[11:0]» rs1 funct3 rd opcode _ =>
-    UInt32.mk <| «imm[11:0]» ++ rs1 ++ funct3 ++ rd ++ opcode
-  | @ofStype «imm[11:5]» rs2 rs1 funct3 «imm[4:0]» opcode _ =>
-    UInt32.mk <| «imm[11:5]» ++ rs2 ++ rs1 ++ funct3 ++ «imm[4:0]» ++ opcode
-  | @ofBtype «imm[12|10:5]» rs2 rs1 funct3 «imm[4:1|11]» opcode _ =>
-    UInt32.mk <| «imm[12|10:5]» ++ rs2 ++ rs1 ++ funct3 ++ «imm[4:1|11]» ++ opcode
-  | @ofUtype «imm[31:12]» rd opcode _ =>
-    UInt32.mk <| «imm[31:12]» ++ rd ++ opcode
-  | @ofJtype  «imm[20|10:1|11|19:12]» rd opcode _ =>
-    UInt32.mk <| «imm[20|10:1|11|19:12]» ++ rd ++ opcode
+abbrev toUInt32 (inst : Inst) : UInt32 := inst.toFormat.toUInt32
+
+namespace Pseudo
+
+/-- `rd = rs1` -/
+abbrev MOV rd rs1 := ADDI rd rs1 0
+/-- `rd = if rs1 = 0 then 1 else 0` -/
+abbrev SEQZ rd rs1 := SLTIU rd rs1 1
+/-- `rd = ~~~rs1` -/
+abbrev NOT rd rs1 := XORI rd rs1 (-1 : Int)
+/-- `rd = if rs2 ≠ 0 then 1 else 0` -/
+abbrev SNEZ rd rs2 := SLTU rd .zero rs2
+/-- 2.4.3. NOP Instruction -/
+abbrev NOP := ADDI .zero .zero 0
+/-- Unconditional jump -/
+abbrev J offset := JAL .zero offset
+
+end Pseudo
+
+namespace Hint
+
+abbrev NTL.P1   := ADD .zero .zero (.x 2)
+abbrev NTL.PALL := ADD .zero .zero (.x 3)
+abbrev NTL.S1   := ADD .zero .zero (.x 4)
+abbrev NTL.ALL  := ADD .zero .zero (.x 5)
+abbrev PAUSE    := FENCE 0b0001 0b0000
+
+end Hint
 
 /-- Instruction decoder. -/
 def fromUInt32 : UInt32 → Option Inst := fun ⟨op⟩ =>
-  let funct7 : BitVec  7 := op.extractLsb' 25 _
-  let msbs12 : BitVec 12 := op.extractLsb' 20 _
-  let rs2    : BitVec  5 := op.extractLsb' 20 _
-  let rs1    : BitVec  5 := op.extractLsb' 15 _
-  let msbs20 : BitVec 20 := op.extractLsb' 12 _
-  let funct3 : BitVec  3 := op.extractLsb' 12 _
-  let rd     : BitVec  5 := op.extractLsb'  7 _
-  let opcode : BitVec  7 := op.extractLsb'  0 _
+  let funct7 : BitVec  7 := op.extractLsb 31 25
+  let msbs12 : BitVec 12 := op.extractLsb 31 20
+  let rs2    : BitVec  5 := op.extractLsb 24 20
+  let rs1    : BitVec  5 := op.extractLsb 19 15
+  let msbs20 : BitVec 20 := op.extractLsb 31 12
+  let funct3 : BitVec  3 := op.extractLsb 14 12
+  let rd     : BitVec  5 := op.extractLsb 11  7
+  let opcode : BitVec  7 := op.extractLsb  6  0
   match opcode with
-  | 0b1101111 => ofJtype <| JAL   msbs20 rd
-  | 0b0110111 => ofUtype <| LUI   msbs20 rd
-  | 0b0010111 => ofUtype <| AUIPC msbs20 rd
+  | 0b1101111 =>
+    let offset : BitVec 20 :=
+      msbs20.extractLsb 19 19 ++ msbs20.extractLsb  7 0 ++
+      msbs20.extractLsb  8  8 ++ msbs20.extractLsb 18 9
+    JAL rd offset
+  | 0b0110111 => LUI   rd msbs20
+  | 0b0010111 => AUIPC rd msbs20
   | 0b1100011 =>
+    let offset : BitVec 12 :=
+      funct7.extractLsb 6 6 ++ rd.extractLsb 0 0 ++
+      funct7.extractLsb 5 0 ++ rd.extractLsb 3 0
     match funct3 with
-    | 0b000 => ofBtype <| BEQ  funct7 rs2 rs1 rd
-    | 0b001 => ofBtype <| BNE  funct7 rs2 rs1 rd
-    | 0b100 => ofBtype <| BLT  funct7 rs2 rs1 rd
-    | 0b101 => ofBtype <| BGE  funct7 rs2 rs1 rd
-    | 0b110 => ofBtype <| BLTU funct7 rs2 rs1 rd
-    | 0b111 => ofBtype <| BGEU funct7 rs2 rs1 rd
+    | 0b000 => BEQ  rs1 rs2 offset
+    | 0b001 => BNE  rs1 rs2 offset
+    | 0b100 => BLT  rs1 rs2 offset
+    | 0b101 => BGE  rs1 rs2 offset
+    | 0b110 => BLTU rs1 rs2 offset
+    | 0b111 => BGEU rs1 rs2 offset
     | _ => none
   | 0b0100011 =>
+    let offset : BitVec 12 := funct7 ++ rd
     match funct3 with
-    | 0b000 => ofStype <| SB funct7 rs2 rs1 rd
-    | 0b001 => ofStype <| SH funct7 rs2 rs1 rd
-    | 0b010 => ofStype <| SW funct7 rs2 rs1 rd
+    | 0b000 => SB rs1 rs2 offset
+    | 0b001 => SH rs1 rs2 offset
+    | 0b010 => SW rs1 rs2 offset
     | _ => none
   | 0b1100111 =>
     match funct3 with
-    | 0b000 => ofItype <| JALR msbs12 rs1 rd
+    | 0b000 => JALR rs1 rd msbs12
     | _ => none
   | 0b0000011 =>
     match funct3 with
-    | 0b000 => ofItype <| LB  msbs12 rs1 rd
-    | 0b001 => ofItype <| LH  msbs12 rs1 rd
-    | 0b010 => ofItype <| LW  msbs12 rs1 rd
-    | 0b100 => ofItype <| LBU msbs12 rs1 rd
-    | 0b101 => ofItype <| LHU msbs12 rs1 rd
+    | 0b000 => LB  rd rs1 msbs12
+    | 0b001 => LH  rd rs1 msbs12
+    | 0b010 => LW  rd rs1 msbs12
+    | 0b100 => LBU rd rs1 msbs12
+    | 0b101 => LHU rd rs1 msbs12
     | _ => none
   | 0b0001111 =>
-    let fm   : BitVec 4 := msbs12.extractLsb' 8 _
-    let pred : BitVec 4 := msbs12.extractLsb' 4 _
-    let succ : BitVec 4 := msbs12.extractLsb' 0 _
+    let fm   : BitVec 4 := msbs12.extractLsb 11 8
+    let pred : BitVec 4 := msbs12.extractLsb  7 4
+    let succ : BitVec 4 := msbs12.extractLsb  3 0
     match fm, pred, succ with
-    | 0b0000, 0b0001, 0b0000 => ofItype PAUSE
-    | 0b1000, 0b0011, 0b0011 => ofItype FENCE.TSO
-    | _, _, _ => ofItype <| FENCE fm pred succ rs1 rd
+    | 0b1000, 0b0011, 0b0011 => FENCE.TSO
+    | _, _, _ => FENCE pred succ
   | 0b1110011 =>
     match msbs12 with
-    | 0 => ofItype ECALL
-    | 1 => ofItype EBREAK
+    | 0 => ECALL
+    | 1 => EBREAK
     | _ => none
   | 0b0010011 =>
-    match funct3 with
-    | 0b000 => ofItype <| ADDI  msbs12 rs1 rd
-    | 0b001 =>
-      match funct7 with
-      | 0b0000000 => ofRtype <| SLLI rs2 rs1 rd
-      | _ => none
-    | 0b010 => ofItype <| SLTI  msbs12 rs1 rd
-    | 0b011 => ofItype <| SLTIU msbs12 rs1 rd
-    | 0b100 => ofItype <| XORI  msbs12 rs1 rd
-    | 0b101 =>
-      match funct7 with
-      | 0b0000000 => ofRtype <| SRLI rs2 rs1 rd
-      | 0b0100000 => ofRtype <| SRAI rs2 rs1 rd
-      | _ => none
-    | 0b110 => ofItype <| ORI   msbs12 rs1 rd
-    | 0b111 => ofItype <| ANDI  msbs12 rs1 rd
-    | _ => none
+    match funct3, funct7 with
+    | 0b000,  _ => ADDI  rd rs1 msbs12
+    | 0b001,  0 => SLLI  rd rs1 rs2
+    | 0b010,  _ => SLTI  rd rs1 msbs12
+    | 0b011,  _ => SLTIU rd rs1 msbs12
+    | 0b100,  _ => XORI  rd rs1 msbs12
+    | 0b101,  0 => SRLI  rd rs1 rs2
+    | 0b101, 32 => SRAI  rd rs1 rs2
+    | 0b110,  _ => ORI   rd rs1 msbs12
+    | 0b111,  _ => ANDI  rd rs1 msbs12
+    | _, _ => none
   | 0b0110011 =>
     match funct3, funct7 with
-    | 0b000, 0b0000000 => ofRtype <| ADD  rs2 rs1 rd
-    | 0b000, 0b0100000 => ofRtype <| SUB  rs2 rs1 rd
-    | 0b001, 0b0000000 => ofRtype <| SLL  rs2 rs1 rd
-    | 0b010, 0b0000000 => ofRtype <| SLT  rs2 rs1 rd
-    | 0b011, 0b0000000 => ofRtype <| SLTU rs2 rs1 rd
-    | 0b100, 0b0000000 => ofRtype <| XOR  rs2 rs1 rd
-    | 0b101, 0b0000000 => ofRtype <| SRL  rs2 rs1 rd
-    | 0b101, 0b0100000 => ofRtype <| SRA  rs2 rs1 rd
-    | 0b110, 0b0000000 => ofRtype <| OR   rs2 rs1 rd
-    | 0b111, 0b0000000 => ofRtype <| AND  rs2 rs1 rd
+    | 0b000,  0 => ADD  rd rs1 rs2
+    | 0b000, 32 => SUB  rd rs1 rs2
+    | 0b001,  0 => SLL  rd rs1 rs2
+    | 0b010,  0 => SLT  rd rs1 rs2
+    | 0b011,  0 => SLTU rd rs1 rs2
+    | 0b100,  0 => XOR  rd rs1 rs2
+    | 0b101,  0 => SRL  rd rs1 rs2
+    | 0b101, 32 => SRA  rd rs1 rs2
+    | 0b110,  0 => OR   rd rs1 rs2
+    | 0b111,  0 => AND  rd rs1 rs2
     | _, _ => none
   | _ => none
 
